Tweak

theories/Sem.v
@@ -8,7 +8,7 @@ Set Implicit Arguments.
 Inductive sort: Type :=
 | angelic
 | demonic
-| final
+| final (retv: val)
 | vis
 .
 
@@ -30,49 +30,3 @@ Record semantics : Type := Semantics_gen {
   wf_demonic: forall st0 ev st1 (VIS: state_sort st0 = demonic) (STEP: step st0 ev st1), ev = None;
 }.
 
-Section SEM.
-Variable L: semantics.
-
-Inductive tstar (st0: L.(state)) (P: L.(state) -> Prop): Prop :=
-| tstar_refl
-    (PROP: P st0)
-  :
-    tstar st0 P
-| tstar_demonic
-    (SRT: L.(state_sort) st0 = demonic)
-    (STEP: exists st1 (STEP: L.(step) st0 None st1), <<TL: tstar st1 P>>)
-  :
-    tstar st0 P
-| tstar_angelic
-    (SRT: L.(state_sort) st0 = angelic)
-    (STEP: forall st1 (STEP: L.(step) st0 None st1), <<TL: tstar st1 P>>)
-  :
-    tstar st0 P
-.
-
-Theorem tstar_ind2 :
-forall P : state L -> (state L -> Prop) -> Prop,
-(forall (st0 : state L) (P0 : state L -> Prop), P0 st0 -> P st0 P0) ->
-(forall (st0 : state L) (P0 : state L -> Prop),
- state_sort L st0 = demonic ->
- (exists (st1 : state L) (_ : step L st0 None st1), <<TL: tstar st1 P0 >> /\ <<IH: P st1 P0>>) -> P st0 P0) ->
-(forall (st0 : state L) (P0 : state L -> Prop),
- state_sort L st0 = angelic ->
- (forall st1 : state L, step L st0 None st1 -> <<TL: tstar st1 P0 >>) ->
- (forall st1 : state L, step L st0 None st1 -> P st1 P0) -> P st0 P0) ->
-forall (st0 : state L) (P0 : state L -> Prop), tstar st0 P0 -> P st0 P0.
-Proof.
-  fix IH 7. i.
-  inv H2.
-  - eapply H; eauto.
-  - eapply H0; eauto. des. esplits; eauto. eapply IH; eauto.
-  - eapply H1; eauto. ii. exploit STEP; eauto. i. esplits; eauto. eapply IH; eauto.
-Qed.
-
-Definition is_leaf (st0: L.(state)): bool :=
-  match L.(state_sort) st0 with
-  | final | vis => true
-  | _ => false
-  end
-.
-End SEM.
