theories/ModSem.v
@@ -1,0 +1,31 @@
+Require Import sflib.
+Require Import Universe.
+Require Import Sem.
+Require Import Behavior.
+From Paco Require Import paco.
+Require Import RelationClasses List.
+Require Import ClassicalChoice PropExtensionality FunctionalExtensionality.
+Require Import Program.
+Require Import String.
+
+Set Implicit Arguments.
+
+Module ModSem.
+
+  Inductive sort: Type :=
+  | angelic
+  | demonic
+  | final (retv: val)
+  | vis
+  | at_external (args: list val)
+  .
+
+  Record t: Type := mk {
+    state: Type;
+    local_data: Type;
+    step (st0: state) (ev: option event) (st1: state): Prop;
+    state_sort: state -> sort;
+  }
+  .
+
+End ModSem.
